isabelle/interpreter/CoreValue.thy
@@ -234,6 +234,12 @@ next
   qed auto
 qed
 
+(* value_has_type does not depend on TE_ProofGoal (corollary of the env
+   congruence: a TE_ProofGoal update touches none of the read fields). *)
+lemma value_has_type_TE_ProofGoal_irrelevant [simp]:
+  "value_has_type (env \<lparr> TE_ProofGoal := g \<rparr>) val ty = value_has_type env val ty"
+  by (rule value_has_type_cong_env) simp_all
+
 
 (* A weaker congruence lemma for value_has_type. Instead of requiring that the
    two environments agree on TE_TypeVars and TE_RuntimeTypeVars, it asks only
